feat (sorting) first steps in quicksort_scheme

thys/examples/sorting/Sorting_Quicksort_Scheme.thy
@@ -2,6 +2,10 @@ theory Sorting_Quicksort_Scheme
 imports Sorting_Setup Sorting_Partially_Sorted
 begin
 
+  
+
+
+
 
   abbreviation "is_threshold \<equiv> 16::nat"
 
@@ -9,160 +13,358 @@ begin
 
     definition "partition1_spec xs \<equiv> doN { 
       ASSERT (length xs \<ge> 4); 
-      SPEC (\<lambda>(xs1,xs2). mset xs = mset xs1 + mset xs2 \<and> xs1\<noteq>[] \<and> xs2\<noteq>[] \<and> slice_LT (\<^bold>\<le>) xs1 xs2)
+      SPEC (\<lambda>(xs1,xs2). mset xs = mset xs1 + mset xs2 \<and> xs1\<noteq>[] \<and> xs2\<noteq>[] \<and> slice_LT (\<^bold>\<le>) xs1 xs2) (\<lambda>_. cost ''partition'' (enat (length xs)))
     }"
-    definition introsort_aux1 :: "'a list \<Rightarrow> nat \<Rightarrow> 'a list nres" where "introsort_aux1 xs d \<equiv> RECT (\<lambda>introsort_aux1 (xs,d). doN {
-      if length xs > is_threshold then doN {
-        if d=0 then
-          SPEC (sort_spec (\<^bold><) xs)
-        else doN {
+definition introsort_aux1 :: "(nat \<Rightarrow> nat) \<Rightarrow> 'a list \<Rightarrow> nat \<Rightarrow> ('a list,_) nrest" where "introsort_aux1 tf xs d \<equiv> RECT' (\<lambda>introsort_aux1 (xs,d). doN {
+      lxs \<leftarrow> SPECT [length xs \<mapsto> cost ''list_length'' 1];
+      b \<leftarrow> SPECc2 ''lt'' (<) is_threshold (length xs);
+      MIf b (doN {
+        b2 \<leftarrow> SPECc2 ''eq'' (=) d 0;
+        MIf b2 (
+          SPEC (sort_spec (\<^bold><) xs) (\<lambda>_. cost ''slice_sort_p'' (enat (tf (length xs))))
+        )( doN {
           (xs1,xs2)\<leftarrow>partition1_spec xs;
           xs1 \<leftarrow> introsort_aux1 (xs1,d-1);
           xs2 \<leftarrow> introsort_aux1 (xs2,d-1);
-          RETURN (xs1@xs2)
-        }
+          SPECc2 ''list_append'' (@) xs1 xs2
+        })
       }
-      else
-        RETURN xs
+      ) (
+        RETURN xs )
     }) (xs,d)"
     
     lemma slice_strict_LT_imp_LE: "slice_LT (\<^bold><) xs ys \<Longrightarrow> slice_LT (le_by_lt (\<^bold><)) xs ys"  
       apply (erule slice_LT_mono)
       by (meson le_by_lt_def wo_less_asym)
-      
-    lemma introsort_aux1_correct: "introsort_aux1 xs d \<le> SPEC (\<lambda>xs'. mset xs' = mset xs \<and> part_sorted_wrt (le_by_lt (\<^bold><)) is_threshold xs')"
+
+
+
+definition introsort_aux_cost :: "_ \<Rightarrow> 'a list * nat \<Rightarrow> (char list, enat) acost"
+  where "introsort_aux_cost tf = (\<lambda>(xs, d). lift_acost (
+        cost ''if'' (2^(d+1)-1) + cost ''eq'' (2^(d+1)-1) + cost ''if'' (2^(d+1)-1)
+         + cost ''lt'' (2^(d+1)-1) + cost ''call'' ((2^(d+1)-1)) 
+        + cost ''list_length'' (2^(d+1)-1) 
+        + cost ''list_append'' (2^(d+1)-1) 
+        +   cost ''slice_sort_p'' (tf (length xs)) + cost ''partition'' (d*(length xs))
+         )
+        )"
+ 
+
+lemma haha: "b>0 \<Longrightarrow> Suc (Suc (4 * 2 ^ (b - Suc 0) - Suc (Suc 0))) \<le> 2 * 2 ^ b"
+proof -
+  assume "b>0"
+  then obtain b' where b: "b=b'+1"  
+    by (metis Groups.add_ac(2) Suc_eq_plus1_left Suc_pred)  
+  have ge2: "4 * (2::nat) ^ (b') \<ge> 2" by auto
+  have "Suc (Suc (4 * 2 ^ (b - Suc 0) - Suc (Suc 0)))
+      = Suc (Suc (4 * 2 ^ (b') - Suc (Suc 0)))" using b by simp
+  also have "\<dots> =  2 + (4*2^b' - 2)" by presburger
+  also have "\<dots> = 4*2^b'" using ge2 by auto
+  also have "\<dots> = 2*2^(b'+1)" by simp
+  also have "\<dots> = 2*2^(b)" using b by simp
+  finally
+    show ?thesis by simp
+  qed
+
+lemma ha: "b>0 \<Longrightarrow> Suc (Suc (8 * 2 ^ (b - Suc 0) - Suc (Suc 0))) \<le> 4 * 2 ^ b"
+proof -
+  assume "b>0"
+  then obtain b' where b: "b=b'+1"  
+    by (metis Groups.add_ac(2) Suc_eq_plus1_left Suc_pred)  
+  have ge2: "4 * (2::nat) ^ (b') \<ge> 2" by auto
+  have "Suc (Suc (4 * 2 ^ (b - Suc 0) - Suc (Suc 0)))
+      = Suc (Suc (4 * 2 ^ (b') - Suc (Suc 0)))" using b by simp
+  also have "\<dots> =  2 + (4*2^b' - 2)" by presburger
+  also have "\<dots> = 4*2^b'" using ge2 by auto
+  also have "\<dots> = 2*2^(b'+1)" by simp
+  also have "\<dots> = 2*2^(b)" using b by simp
+  finally
+    show ?thesis by simp
+  qed
+ 
+
+lemma argh: "b>0 \<Longrightarrow> 4 * 2 ^ (b - Suc 0) - Suc 0 \<le> 2 * 2 ^ b - Suc 0"
+proof -
+  assume "b>0"
+  then obtain b' where b: "b=b'+1"  
+    by (metis Groups.add_ac(2) Suc_eq_plus1_left Suc_pred)  
+  then have "4 * 2 ^ (b - Suc 0) - Suc 0 = 4 * 2 ^ ((b'+1) - Suc 0) - Suc 0 "
+    by auto
+  also have "\<dots> = 2 * (2*2^b') - Suc 0" apply simp done
+  also have "\<dots> = 2 * (2^(b'+1)) - Suc 0" apply simp done
+  also have "\<dots> = 2 * 2 ^ b - Suc 0" using b apply simp done
+  finally show ?thesis by simp
+qed
+
+lemma argh2: "b>0 \<Longrightarrow> Suc (4 * 2 ^ (b - Suc 0) - Suc (Suc 0)) \<le> 2 * 2 ^ b - Suc 0"
+proof -
+  assume "b>0"
+  then obtain b' where b: "b=b'+1"  
+    by (metis Groups.add_ac(2) Suc_eq_plus1_left Suc_pred)  
+  then have "Suc (4 * 2 ^ (b - Suc 0) - Suc (Suc 0)) = Suc (4 * 2 ^ ((b'+1) - Suc 0) - Suc (Suc 0) )"
+    by auto
+  also have "\<dots> = Suc (2 * (2*2^b') - Suc (Suc 0))" apply simp done
+  also have "\<dots> = (2 * (2*2^b') - Suc 0)" apply(subst Suc_diff_Suc) apply auto
+    by (simp add: Suc_lessI)
+  also have "\<dots> = 2 * (2^(b'+1)) - Suc 0" apply simp done
+  also have "\<dots> = 2 * 2 ^ b - Suc 0" using b apply simp done
+  finally show ?thesis by simp
+qed
+
+lemma z: "b>0 \<Longrightarrow> (b - Suc 0) * A + (b - Suc 0) * B + (B + A) = b*(A+B)"
+proof -
+  assume "b>0"
+  then obtain b' where b: "b=b'+1"  
+    by (metis Groups.add_ac(2) Suc_eq_plus1_left Suc_pred)  
+  then have "(b - Suc 0) * A + (b - Suc 0) * B + (B + A)
+      = (b') * A + (b') * B + (B + A)" by simp
+  also have "\<dots> = (b'+1) * (B+A)" by (auto simp: ring_distribs)
+  also have "\<dots> = b * (B+A)" using b by simp
+  finally show ?thesis by simp
+qed
+
+lemma lengths_sums_if_msets_do: "mset a = mset b + mset c \<Longrightarrow> length a = length b + length c"
+    by (metis add.commute length_append less_or_eq_imp_le mset_append mset_eq_length)  
+
+lemma zz: "Suc 0 \<le> 4 * 2 ^ b - Suc (Suc 0)"
+proof -
+  show ?thesis 
+    apply(rule add_le_imp_le_diff)  apply simp
+    apply(rule order.trans[where b="4 * 2 ^ 0"])
+     apply simp
+    apply  simp
+    done      
+qed
+
+
+  lemma introsort_aux1_correct:
+    assumes tf_suplinear: "\<And>a b c. a+b\<le>c \<Longrightarrow> tf a + tf b \<le> tf c"
+    shows 
+   "introsort_aux1 tf xs d \<le> SPEC (\<lambda>xs'. mset xs' = mset xs \<and> part_sorted_wrt (le_by_lt (\<^bold><)) is_threshold xs') (\<lambda>_. introsort_aux_cost tf (xs, d))"
     
       unfolding introsort_aux1_def partition1_spec_def sort_spec_def
-      
-      apply (refine_vcg RECT_rule_arb[where V="measure (\<lambda>(xs,d). d+1)" and pre="\<lambda>xss (xs',d). xss=xs'"])
+ 
+
+      apply (rule RECT'_rule_arb[where V="measure (\<lambda>(xs,d). d+1)" and pre="\<lambda>xss (xs',d). xss=xs'"])
+      apply refine_mono
       apply (all \<open>(auto intro: sorted_wrt_imp_part_sorted part_sorted_wrt_init; fail)?\<close>)
-      apply (rule order_trans)
-      apply rprems
-      applyS (simp)
-      subgoal by auto
-      apply refine_vcg
+
+      unfolding SPEC_REST_emb'_conv SPECc2_alt
+      subgoal premises prems for f xss x
+      apply(rule gwp_specifies_I) 
+        apply(refine_vcg \<open>-\<close> rules: prems(1)[THEN gwp_specifies_rev_I, THEN gwp_conseq_0])
+        thm prems(1)[THEN gwp_specifies_rev_I, THEN gwp_conseq_0]
+        using  prems(2)
+      subgoal unfolding emb'_def apply auto
+        subgoal  by (simp add: sorted_wrt_imp_part_sorted)
+        subgoal unfolding introsort_aux_cost_def
+            apply (simp add: lift_acost_propagate lift_acost_cost)
+          apply sc_solve by (auto simp: one_enat_def)
+        done
+            apply simp apply simp
+          apply simp apply simp
       subgoal
-        apply (rule order_trans)
-        apply rprems
-        applyS simp
-        subgoal by auto
-        apply refine_vcg  
-        subgoal by auto
-        subgoal
-          apply clarsimp
+        apply (auto simp add: emb'_def handy_if_lemma)
+        
+        subgoal  using prems(2) by simp  
+        subgoal 
           apply (rule part_sorted_concatI; assumption?) 
           apply (subst slice_LT_mset_eq1, assumption)
           apply (subst slice_LT_mset_eq2, assumption)
           using le_by_lt by blast
+        subgoal premises p
+          unfolding introsort_aux_cost_def
+          using p(3,8)
+          apply (simp add: lift_acost_propagate lift_acost_cost)
+          apply sc_solve_debug apply safe apply(all \<open>((auto simp: sc_solve_debug_def),fail)?\<close>)
+          subgoal (* append *) unfolding sc_solve_debug_def by (simp add: one_enat_def argh) 
+          subgoal (* partition *)
+            unfolding sc_solve_debug_def
+            apply(drule lengths_sums_if_msets_do)
+            apply auto apply(simp only: z) apply simp done
+          subgoal unfolding sc_solve_debug_def apply (simp add: one_enat_def argh) 
+            apply(rule add_le_imp_le_diff) apply simp apply(rule ha) by simp 
+          subgoal unfolding sc_solve_debug_def
+            apply (simp add: one_enat_def)
+            apply(rule tf_suplinear)
+            by (metis add.commute length_append less_or_eq_imp_le mset_append mset_eq_length)  
+
+          subgoal unfolding sc_solve_debug_def
+            by (simp add: one_enat_def argh)
+          subgoal unfolding sc_solve_debug_def apply (simp add: one_enat_def argh) 
+            apply(rule add_le_imp_le_diff) apply simp apply(rule haha) by simp 
+          subgoal (* lt *) unfolding sc_solve_debug_def by (simp add: one_enat_def argh) 
+          subgoal (* call *) unfolding sc_solve_debug_def apply (simp add: one_enat_def ) 
+            apply(rule argh2) by simp 
+          done
+        done
+      subgoal by auto
+      subgoal
+        using prems(2) apply (auto simp add: emb'_def handy_if_lemma)
+        subgoal by (simp add: part_sorted_wrt_init)
+        subgoal unfolding introsort_aux_cost_def apply (simp add: lift_acost_propagate lift_acost_cost)
+          apply sc_solve apply (auto simp: one_enat_def)
+          subgoal 
+            by(rule zz)
+          subgoal  
+            by (smt Suc_leI Suc_pred le_SucE mult_pos_pos n_not_Suc_n numeral_2_eq_2 one_eq_mult_iff pos2 zero_less_power)  
+          done
         done
       done
-    
+    done
+ 
       
     definition "partition2_spec xs \<equiv> doN { 
       ASSERT (length xs \<ge> 4); 
-      SPEC (\<lambda>(xs',i). mset xs' = mset xs \<and> 0<i \<and> i<length xs \<and> slice_LT (\<^bold>\<le>) (take i xs') (drop i xs'))
+      SPEC (\<lambda>(xs',i). mset xs' = mset xs \<and> 0<i \<and> i<length xs \<and> slice_LT (\<^bold>\<le>) (take i xs') (drop i xs')) (\<lambda>_. cost ''partition'' (enat (length xs)))
     }"
       
-    lemma partition2_spec_refine: "(xs,xs')\<in>Id \<Longrightarrow> partition2_spec xs \<le>\<Down>(br (\<lambda>(xs,i). (take i xs, drop i xs)) (\<lambda>(xs,i). 0<i \<and> i<length xs)) (partition1_spec xs')"
+    lemma partition2_spec_refine: "(xs,xs')\<in>Id \<Longrightarrow> partition2_spec xs \<le>\<Down>(br (\<lambda>(xs,i). (take i xs, drop i xs)) (\<lambda>(xs,i). 0<i \<and> i<length xs)) (timerefine TId (partition1_spec xs'))"
       unfolding partition1_spec_def partition2_spec_def
-      apply (refine_vcg RES_refine)
-      by (auto dest: mset_eq_length simp: in_br_conv simp flip: mset_append)
+      apply (intro refine0 SPEC_both_refine)
+       apply (auto dest: mset_eq_length simp: in_br_conv simp flip: mset_append)
+      subgoal
+        using mset_eq_length by fastforce
+      subgoal
+        using mset_eq_length by force
+      done
       
-    definition introsort_aux2 :: "'a list \<Rightarrow> nat \<Rightarrow> 'a list nres" where "introsort_aux2 xs d \<equiv> RECT (\<lambda>introsort_aux (xs,d). doN {
-      if length xs > is_threshold then doN {
-        if d=0 then
-          SPEC (sort_spec (\<^bold><) xs)
-        else doN {
+    definition introsort_aux2 :: "(nat \<Rightarrow> nat) \<Rightarrow> 'a list \<Rightarrow> nat \<Rightarrow> ('a list,_) nrest" where "introsort_aux2 tf xs d \<equiv> RECT' (\<lambda>introsort_aux (xs,d). doN {
+      lxs \<leftarrow> SPECT [length xs \<mapsto> cost ''list_length'' 1];
+      b \<leftarrow> SPECc2 ''lt'' (<) is_threshold (length xs);
+      MIf b (doN {
+        b2 \<leftarrow> SPECc2 ''eq'' (=) d 0;
+        MIf b2 (
+          SPEC (sort_spec (\<^bold><) xs) (\<lambda>_. cost ''slice_sort_p'' (enat (tf (length xs))))
+        )( doN {
           (xs,m)\<leftarrow>partition2_spec xs;
           ASSERT (m\<le>length xs);
           xs1 \<leftarrow> introsort_aux (take m xs,d-1);
           xs2 \<leftarrow> introsort_aux (drop m xs,d-1);
-          RETURN (xs1@xs2)
-        }
+          SPECc2 ''list_append'' (@) xs1 xs2
+        })
       }
-      else
-        RETURN xs
+      ) (
+        RETURN xs )
     }) (xs,d)"
-      
-    lemma introsort_aux2_refine: "introsort_aux2 xs d \<le>\<Down>Id (introsort_aux1 xs d)"  
+
+    lemma introsort_aux2_refine: "introsort_aux2 tf xs d \<le>\<Down>Id (timerefine TId (introsort_aux1 tf xs d))"  
       unfolding introsort_aux2_def introsort_aux1_def
-      apply (refine_rcg partition2_spec_refine)
+      apply (refine_rcg partition2_spec_refine SPEC_both_refine MIf_refine SPECc2_refine RECT'_refine_t bindT_refine_easy)
       apply refine_dref_type
-      apply (auto simp: in_br_conv)
+      apply refine_mono
+      apply (auto simp: in_br_conv cost_n_leq_TId_n)
       done
       
     
     definition "partition3_spec xs l h \<equiv> doN { 
       ASSERT (h-l\<ge>4 \<and> h\<le>length xs); 
-      SPEC (\<lambda>(xs',i). slice_eq_mset l h xs' xs \<and> l<i \<and> i<h \<and> slice_LT (\<^bold>\<le>) (slice l i xs') (slice i h xs')) 
+      SPEC (\<lambda>(xs',i). slice_eq_mset l h xs' xs \<and> l<i \<and> i<h \<and> slice_LT (\<^bold>\<le>) (slice l i xs') (slice i h xs')) (\<lambda>_. cost ''partition'' (enat (h-l)))
     }"
-    
-    lemma partition3_spec_refine: "(xsi,xs) \<in> slice_rel xs\<^sub>0 l h \<Longrightarrow> partition3_spec xsi l h  \<le>\<Down>(slice_rel xs\<^sub>0 l h \<times>\<^sub>r idx_shift_rel l) (partition2_spec xs)"
+ 
+abbreviation "TR_i_aux \<equiv> (TId(''list_append'':=0,''list_length'':=cost ''sub'' 1))"
+
+    lemma partition3_spec_refine: "(xsi,xs) \<in> slice_rel xs\<^sub>0 l h \<Longrightarrow> partition3_spec xsi l h  \<le>\<Down>(slice_rel xs\<^sub>0 l h \<times>\<^sub>r idx_shift_rel l) (timerefine TR_i_aux (partition2_spec xs))"
       unfolding partition3_spec_def partition2_spec_def
-      apply (refine_vcg RES_refine)
-      apply (auto simp: slice_rel_def in_br_conv) [2]
-      apply (clarsimp simp: slice_rel_def in_br_conv)
+      apply (intro refine0 SPEC_both_refine)
+       apply (auto simp: slice_rel_def in_br_conv) [2]
       subgoal for xs'i ii
         apply (rule exI[where x="slice l h xs'i"])
         apply (rule conjI)
         subgoal by (auto simp: slice_eq_mset_def)
         apply (simp add: idx_shift_rel_alt)
-        by (auto simp: slice_eq_mset_def take_slice drop_slice)
+        by (auto simp: slice_eq_mset_def take_slice drop_slice intro!: cost_mono)
       done
 
       
     lemma partition3_spec_refine': "\<lbrakk>(xsi,xs) \<in> slicep_rel l h; xsi'=xsi; l'=l; h'=h\<rbrakk> 
-      \<Longrightarrow> partition3_spec xsi l h  \<le>\<Down>(slice_rel xsi' l' h' \<times>\<^sub>r idx_shift_rel l') (partition2_spec xs)"
+      \<Longrightarrow> partition3_spec xsi l h  \<le>\<Down>(slice_rel xsi' l' h' \<times>\<^sub>r idx_shift_rel l') (timerefine TR_i_aux (partition2_spec xs))"
       unfolding partition3_spec_def partition2_spec_def
-      apply (refine_vcg RES_refine)
-      apply (auto simp: slicep_rel_def in_br_conv) [2]
-      apply (clarsimp simp: slice_rel_def slicep_rel_def in_br_conv)
+      apply (intro refine0 SPEC_both_refine )
+      apply (auto simp: slicep_rel_def in_br_conv) [2] 
       subgoal for xs'i ii
         apply (rule exI[where x="slice l h xs'i"])
         apply (rule conjI)
         subgoal by (auto simp: slice_eq_mset_def)
         apply (simp add: idx_shift_rel_alt)
-        by (auto simp: slice_eq_mset_def take_slice drop_slice)
+        apply (auto simp: slice_eq_mset_def take_slice drop_slice intro!: cost_mono)
+        by (smt less_or_eq_imp_le less_trans slice_eq_mset_alt slice_eq_mset_def slice_in_slice_rel slice_rel_alt)
       done
       
+definition "slice_sort_specT T lt xs\<^sub>0 l h \<equiv> doN {
+    ASSERT (l\<le>h \<and> h\<le>length xs\<^sub>0);
+    SPEC (\<lambda>xs. length xs = length xs\<^sub>0 \<and> take l xs = take l xs\<^sub>0 \<and> drop h xs = drop h xs\<^sub>0 \<and> sort_spec lt (Misc.slice l h xs\<^sub>0) (Misc.slice l h xs))
+         (\<lambda>_. T)
+  }"
       
-    definition introsort_aux3 :: "'a list \<Rightarrow> nat \<Rightarrow> nat \<Rightarrow> nat \<Rightarrow> 'a list nres" where "introsort_aux3 xs l h d 
-    \<equiv> RECT (\<lambda>introsort_aux (xs,l,h,d). doN {
+    definition introsort_aux3 :: "(nat \<Rightarrow> nat) \<Rightarrow> 'a list \<Rightarrow> nat \<Rightarrow> nat \<Rightarrow> nat \<Rightarrow> ('a list,_) nrest" where "introsort_aux3 tf xs l h d 
+    \<equiv> RECT' (\<lambda>introsort_aux (xs,l,h,d). doN {
         ASSERT (l\<le>h);
-        if h-l > is_threshold then doN {
-          if d=0 then
-            slice_sort_spec (\<^bold><) xs l h
-          else doN {
+        lxs \<leftarrow> SPECc2 ''sub'' (-) h l;
+        b \<leftarrow> SPECc2 ''lt'' (<) is_threshold (length xs);
+        MIf b (doN {
+          b2 \<leftarrow> SPECc2 ''eq'' (=) d 0;
+          MIf b2 (
+            slice_sort_specT (cost ''slice_sort_p'' (enat (tf (length xs)))) (\<^bold><) xs l h
+          )( doN {
             (xs,m)\<leftarrow>partition3_spec xs l h;
             xs \<leftarrow> introsort_aux (xs,l,m,d-1);
             xs \<leftarrow> introsort_aux (xs,m,h,d-1);
             RETURN xs
-          }
+          })
         }
-        else
-          RETURN xs
+        ) (
+          RETURN xs )
       }) (xs,l,h,d)"
-      
-    lemma introsort_aux3_refine: "(xsi,xs)\<in>slicep_rel l h \<Longrightarrow> introsort_aux3 xsi l h d \<le> \<Down>(slice_rel xsi l h) (introsort_aux2 xs d)"  
+
+
+
+
+corollary my_slice_sort_spec_refine_sort': "\<lbrakk>(xsi,xs) \<in> slicep_rel l h; xsi'=xsi; l'=l; h'=h\<rbrakk> \<Longrightarrow> slice_sort_specT (T xsi) lt xsi l h \<le>\<Down>(slice_rel xsi' l' h') (timerefine TR_i_aux (SPEC (sort_spec lt xs) (\<lambda>_. T xs)))"
+  sorry
+  
+
+lemma introsort_aux3_refine: "(xsi,xs)\<in>slicep_rel l h
+       \<Longrightarrow> introsort_aux3 tf xsi l h d \<le> \<Down>(slice_rel xsi l h) (timerefine TR_i_aux (introsort_aux2 tf xs d))"  
       unfolding introsort_aux3_def introsort_aux2_def
       
-      supply recref = RECT_dep_refine[where 
+      supply recref = RECT'_dep_refine[where 
           R="\<lambda>_. {((xsi::'a list, l, h, di::nat), (xs, d)). (xsi, xs) \<in> slicep_rel l h \<and> di=d}" and
           S="\<lambda>_ (xsi::'a list, l, h, di::nat). slice_rel xsi l h" and
           arb\<^sub>0 = "()"
           ]
-
-      apply (refine_rcg 
+      unfolding SPECc2_def
+      apply (refine_rcg bindT_refine_easy MIf_refine
         recref 
         partition3_spec_refine'
-        slice_sort_spec_refine_sort'
-        ; (rule refl)?
+        my_slice_sort_spec_refine_sort'
+        ; (intro refl wfR''_TId wfR''_upd sp_TId struct_preserving_upd_I )?
         )
+            apply refine_mono 
 
-      subgoal by auto
-      subgoal by auto
+      apply(simp_all add: timerefineA_update_cost timerefineA_update_apply_same_cost)
+
+                apply refine_dref_type
+               apply auto
+      prefer 7
+      subgoal unfolding RETURNT_alt apply(rule SPECT_refine_t) 
+        subgoal sorry
+        by (simp add: timerefineA_update_apply_same_cost)
+ 
       subgoal by (auto simp: slicep_rel_def)
       subgoal by (auto simp: slicep_rel_def)
+      subgoal   sorry
+      subgoal   sorry
+      subgoal premises prems for f f' (* first recursive call *)
+        using prems(2)
+        sorry
+      subgoal premises prems for f f' (* second recursive call *)
+        using prems(2)
+        sorry
+      subgoal by (auto simp: slicep_rel_def)
+      done
+        
+(*
       subgoal by auto
       subgoal by auto
       subgoal by auto
@@ -188,38 +390,53 @@ begin
         done
       subgoal by (auto simp: slice_rel_alt eq_outside_range_triv slicep_rel_def)
       done
-    
+    *)
 
     definition "slice_part_sorted_spec xsi l h \<equiv> doN { ASSERT (l\<le>h \<and> h\<le>length xsi); SPEC (\<lambda>xsi'. 
         eq_outside_range xsi' xsi l h 
       \<and> mset (slice l h xsi') = mset (slice l h xsi) 
-      \<and> part_sorted_wrt (le_by_lt (\<^bold><)) is_threshold (slice l h xsi'))}"
+      \<and> part_sorted_wrt (le_by_lt (\<^bold><)) is_threshold (slice l h xsi')) (\<lambda>_. cost ''slice_part_sorted'' 1)}"
     
-          
-    lemma introsort_aux3_correct: "introsort_aux3 xsi l h d \<le> slice_part_sorted_spec xsi l h"
+
+    term introsort_aux_cost
+
+declare nrest_Rel_mono[trans]
+
+
+definition introsort_aux_cost2 :: "_ \<Rightarrow> 'a list * nat \<Rightarrow> (char list, enat) acost"
+  where "introsort_aux_cost2 tf = (\<lambda>(xs, d). lift_acost (
+        cost ''if'' (2^(d+1)-1) + cost ''eq'' (2^(d+1)-1) + cost ''if'' (2^(d+1)-1)
+         + cost ''lt'' (2^(d+1)-1) + cost ''call'' ((2^(d+1)-1)) 
+        + cost ''sub'' (2^(d+1)-1)  
+        +   cost ''slice_sort_p'' (tf (length xs)) + cost ''partition'' (d*(length xs))
+         )
+        )"
+
+
+    lemma introsort_aux3_correct: "introsort_aux3 tf xsi l h d \<le> timerefine TR_i_aux (timerefine (TId(''slice_part_sorted'':=introsort_aux_cost tf (xsi,d))) (slice_part_sorted_spec xsi l h))"
     proof -
     
 (*      have "(xsi, slice l h xsi) \<in> slicep_rel l h"
         unfolding slicep_rel_def apply auto
         *)
     
-      have A: "\<Down> (slice_rel xsi l h) (SPEC (\<lambda>xs'. mset xs' = mset (slice l h xsi) \<and> part_sorted_wrt (le_by_lt (\<^bold><)) 16 xs'))
+      have A: "\<Down> (slice_rel xsi l h) (SPEC (\<lambda>xs'. mset xs' = mset (slice l h xsi) \<and> part_sorted_wrt (le_by_lt (\<^bold><)) 16 xs')  (\<lambda>_. cost ''slice_part_sorted'' 1))
         \<le> slice_part_sorted_spec xsi l h"
         apply (clarsimp simp: slice_part_sorted_spec_def pw_le_iff refine_pw_simps)
         apply (auto simp: slice_rel_alt  slicep_rel_def)
-        done
+        sorry
     
-      note introsort_aux3_refine[of xsi "slice l h xsi" l h d]
-      also note introsort_aux2_refine
+      note introsort_aux3_refine[of xsi "slice l h xsi" l h tf d]
+      also note introsort_aux2_refine (* TODO: enable rules like nrest_Rel_mono here *)
       also note introsort_aux1_correct
       also note A
-      finally show ?thesis
+      fin ally show ?thesis
         apply (clarsimp simp: slicep_rel_def slice_part_sorted_spec_def)
-        by (auto simp: pw_le_iff refine_pw_simps)
-        
+        apply (auto simp: pw_le_iff refine_pw_simps)
+        sorry
     qed    
       
-
+(*
     text \<open>In the paper, we summarized steps 2 and 3. Here are the relevant lemmas: \<close>        
     lemma partition3_spec_alt: "partition3_spec xs l h = \<Down>(slice_rel xs l h \<times>\<^sub>r Id) (doN { ASSERT (l\<le>h \<and> h\<le>length xs); (xs\<^sub>1,xs\<^sub>2) \<leftarrow> partition1_spec (slice l h xs); RETURN (xs\<^sub>1@xs\<^sub>2, l+length xs\<^sub>1) })"  
       unfolding partition3_spec_def partition1_spec_def
@@ -315,7 +532,7 @@ begin
       subgoal by (auto simp: slice_rel_alt eq_outside_range_triv slicep_rel_def)
       done
       
-      
+      *)
       
       
       
@@ -335,9 +552,11 @@ begin
         RETURN xs
       } else RETURN xs
     }"  
+
+    definition "introsort3_cost n = cost ''slice_sort'' 1 +  cost ''slice_part_sorted'' (enat n)"
     
     
-    lemma introsort3_correct: "introsort3 xs l h \<le> slice_sort_spec (\<^bold><) xs l h"
+    lemma introsort3_correct: "introsort3 xs l h \<le> timerefine (TId(''slice_sort'':=introsort3_cost (h-l))) (slice_sort_spec (\<^bold><) xs l h)"
       apply (cases "l\<le>h \<and> h\<le>length xs")
       subgoal
         apply (cases "1<h-l")
